steel/Learn.Steel.Util.fst
@@ -43,7 +43,7 @@ let vopt0 (b : bool) (v : vprop) : vprop
 
 let vopt_sl  b v = hp_of  (vopt0 b v)
 let vopt_sel b v = sel_of (vopt0 b v)
-let vopt_eq  b v : squash (vopt b v == expanded_vprop (vopt0 b v)) = ()
+let vopt_eq  b v : squash (vopt b v == vprop_group (vopt0 b v)) = ()
 
 let vopt_intro_t #opened (v : vprop)
   : SteelGhost unit opened
@@ -53,7 +53,7 @@ let vopt_intro_t #opened (v : vprop)
     intro_vrewrite v #(vopt_sel_t true v) (fun x -> Some x);
     assert_norm (vopt0 true v == vrewrite v #(vopt_sel_t true v) (fun x -> Some x));
     change_equal_slprop (vrewrite v #(vopt_sel_t true v) (fun x -> Some x)) (vopt0 true v);
-    intro_expanded_vprop (vopt0 true v);
+    intro_vprop_group (vopt0 true v);
     rewrite_vprop (eq_sym (vopt_eq true v))
 
 let vopt_intro_f #opened (v : vprop)
@@ -64,7 +64,7 @@ let vopt_intro_f #opened (v : vprop)
     intro_vrewrite emp #(vopt_sel_t false v) (fun _ -> None);
     assert_norm (vopt0 false v == vrewrite emp #(vopt_sel_t false v) (fun _ -> None));
     change_equal_slprop (vrewrite emp #(vopt_sel_t false v) (fun _ -> None)) (vopt0 false v);
-    intro_expanded_vprop (vopt0 false v);
+    intro_vprop_group (vopt0 false v);
     rewrite_vprop (eq_sym (vopt_eq false v))
 
 let vopt_elim_t #opened (v : vprop)
@@ -73,7 +73,7 @@ let vopt_elim_t #opened (v : vprop)
       (requires fun _ -> True) (ensures fun h0 () h1 -> h0 (vopt true v) == Some (h1 v))
   =
     rewrite_vprop (vopt_eq true v);
-    elim_expanded_vprop (vopt0 true v);
+    elim_vprop_group (vopt0 true v);
     assert_norm (vopt0 true v == vrewrite v #(vopt_sel_t true v) (fun x -> Some x));
     change_equal_slprop (vopt0 true v) (vrewrite v #(vopt_sel_t true v) (fun x -> Some x));
     elim_vrewrite v #(vopt_sel_t true v) (fun x -> Some x)
@@ -84,7 +84,7 @@ let vopt_elim_f #opened (v : vprop)
       (requires fun _ -> True) (ensures fun h0 () h1 -> h0 (vopt false v) == None)
   =
     rewrite_vprop (vopt_eq false v);
-    elim_expanded_vprop (vopt0 false v);
+    elim_vprop_group (vopt0 false v);
     assert_norm (vopt0 false v == vrewrite emp #(vopt_sel_t false v) (fun _ -> None));
     change_equal_slprop (vopt0 false v) (vrewrite emp #(vopt_sel_t false v) (fun _ -> None));
     elim_vrewrite emp #(vopt_sel_t false v) (fun _ -> None)
